\begin{proof}[Solution]
    First, we reparametrize the density function to the parameter $\eta$:
    $$
    \eta = \exp\left(-\frac{t^2}{2\sigma^2}\right) \implies \log(1/\eta) = \frac{t^2}{2\sigma^2} \implies \sigma^2 = \frac{t^2}{2\log(1/\eta)}
    $$
    and 
    $$
    \exp\left(-\frac{x^2}{2\sigma^2}\right) = \exp\left(-\frac{t^2}{2\sigma^2}\frac{x^2}{t^2}\right) = \eta^{x^2/t^2}.
    $$
    Then, the reparametrized density is 
    $$f(x|\eta) = \frac{2}{t^2}\log(1/\eta)x\eta^{x^2/t^2}$$
    and the likelihood function is 
    $$
    L(\eta|\boldsymbol{x}) = \prod_{i=1}^n \frac{2}{t^2}\log(1/\eta)x_i\eta^{x_i^2/t^2} = \frac{2^n}{t^{2n}}\log(1/\eta)^n\left(\prod_{i=1}^n x_i\right) \, \eta^{t^{-2}\sum_{i=1}^n x_i^2}
    $$
\end{proof}